Type.v now compiles

Java/src/Java/Func/Type.v
@@ -3,14 +3,16 @@ Require Import ExtLib.Data.Fun.
 Require Import ExtLib.Data.PList.
 Require Import ExtLib.Data.POption.
 Require Import ExtLib.Tactics.
+Require Import ExtLib.Data.Eq.UIP_trans.
 
 Require Import MirrorCore.TypesI.
 Require Import MirrorCore.MTypes.ModularTypes.
 Require Import MirrorCore.MTypes.ListType.
 Require Import MirrorCore.MTypes.ProdType.
 Require Import MirrorCore.MTypes.BaseType.
-Require Import MirrorCore.syms.SymOneOf.
+Require Import MirrorCore.MTypes.TSymOneOf.
 Require Import MirrorCore.Views.FuncView.
+Require Import MirrorCore.Views.View.
 Require Import MirrorCore.Views.ViewSumN.
 Require Import MirrorCore.MTypes.ListType.
 
@@ -37,133 +39,188 @@ Set Strict Implicit.
 
 Import OneOfType.
 
-Definition typ_map x := 
-  list_to_pmap 
-    (pcons (prod_typ x)
-           (pcons (list_typ x)
-                  (pcons (base_typ x)
-                         (pcons (java_typ x)
-                                pnil)))).
+Definition typ_map := 
+  list_to_pmap
+    (pcons prod_typ (pcons list_typ (pcons base_typ (pcons java_typ pnil)))).
 
-Definition typ' x := OneOfType.OneOf (typ_map x).
+Lemma pmap_lookup'_Empty p : pmap_lookup' Empty p = _None.
+Proof.
+  induction p; simpl in *; try apply IHp. reflexivity.
+Qed.
+(*
+Definition OneOf_Branch_left n l r (H : OneOfF l) : OneOf (Branch n l r).
+Proof.
+  destruct H.
+  exists (xO index0); simpl; apply value0.
+Defined.
+
+Definition OneOf_Branch_right n l r (H : OneOf r) : OneOf (Branch n l r).
+Proof.
+  destruct H.
+  exists (xI index0); simpl; apply value0.
+Defined.
+
+Definition OneOf_Branch_node n l r (H : n) : OneOf (Branch (_Some n) l r).
+Proof.
+  exists xH; simpl; apply H.
+Defined.
+
+
+Definition OneOf_Branch n l r (H : OneOf (Branch (_Some n) l r)) :   
+  n + OneOf l + OneOf r.
+Proof.
+  remember (Branch (_Some n) l r).
+  generalize dependent l; generalize dependent r.
+  induction p; intros; inversion Heqp; subst.
+  destruct H. destruct index0; [right | left; right | left; left; assumption]; simpl in *.
+  exists index0; assumption.
+  exists index0; assumption.
+Defined.
+*)
+Definition typ' := OneOfType.OneOfF typ_map. 
+(*
+Instance TSym_Empty : TSym 
+Proof.
+  split; intros.
+  apply OneOf_Empty in X; destruct X.
+  exfalso. apply OneOf_Empty in a; destruct a.
+Defined.
+
+Instance TSym_Branch n l r 
+         (Hl : TSym (fun x => OneOf (l x)))
+         (Hr : TSym (fun x => OneOf (r x)))
+         (Hn : TSym n) :
+  TSym (fun x => (OneOf (Branch (_Some (n x)) (l x) (r x)))).
+Proof.
+  split; intros.
+  apply OneOf_Branch in X. destruct X as [[X | X] | X].
+  eapply @symbolD in Hn; eassumption.
+  eapply @symbolD in Hl; eassumption.
+  eapply @symbolD in Hr; eassumption.
+  destruct a, b; simpl.
+
+  destruct index0, index1; try (solve [right; intros H; inv_all; subst; inversion x]).
+  + eapply @symbol_dec with (a := mkOneOf _ index0 value0) (b := mkOneOf _ index1 value1) in Hr.
+    destruct Hr; [left | right]; inv_all; subst; [reflexivity|].
+    intros H. apply n1. inv_all. inversion x; subst. 
+    rewrite (uip_trans Pos.eq_dec _ _ x eq_refl) in *. reflexivity.
+  + eapply @symbol_dec with (a := mkOneOf _ index0 value0) (b := mkOneOf _ index1 value1) in Hl.
+    destruct Hl; [left | right]; inv_all; subst; [reflexivity|].
+    intros H. apply n1. inv_all. inversion x; subst. 
+    rewrite (uip_trans Pos.eq_dec _ _ x eq_refl) in *. reflexivity.
+  + eapply @symbol_dec with (a := value0) (b := value1) in Hn.
+    destruct Hn; [left | right]; subst; [reflexivity|].
+    intros H. apply n1. inv_all. inversion x; subst. 
+    rewrite (uip_trans Pos.eq_dec _ _ x eq_refl) in *. reflexivity.
+Defined.
+*)
+Definition TSymAll_typ_map : TSym_All typ_map.
+  repeat first [eapply TSym_All_Branch_None | 
+                eapply TSym_All_Branch_Some; [eapply _ | |] | 
+                eapply TSym_All_Empty]. 
+Defined.
+
+Global Instance TSym_typ' : TSym typ'.
+  apply TSymOneOf. apply TSymAll_typ_map.
+Defined.
+
 Definition typ := mtyp typ'.
 
-Ltac test a b :=   
-  intros;
-  destruct a, b; simpl in *;
-  subst; simpl in *.
-(* *)
-
-
-Ltac test2 :=
-match goal with
-  | a : OneOf _, b : OneOf _ |- _ => 
-    destruct a as [i1 v1];
-      destruct b as [i2 v2];
-      consider (i1 ?[eq] i2); intros; [| apply false]; subst;
-      repeat match goal with
-             | H : match pmap_lookup' Empty ?i with | _Some _ => _ | _None => Empty_set end |- _ => 
-               rewrite pmap_lookup'_Empty in H; destruct H
-             | H1 : match pmap_lookup' _ ?i with | _Some _ => _ | _None => Empty_set end |- _ => 
-               destruct i; simpl in *
-             | v1 : _, v2 : _ |- _ => apply (v1 ?[eq] v2)
-             end
-end.
-
-
-Definition rel_dec_typ' {x : nat} (a b : typ' x) : bool.
-  unfold typ' in *; test2.
+Global Instance RType_typ : RType typ. 
+apply RType_mtyp. apply _.
 Defined.
 
-Ltac eq_dec_right :=
-  let H := fresh "H" in
-    right; intro H; inv_all; congruence.
-
-Instance RelDec_typ : RelDec (@eq typ) := {
-  rel_dec := rel_dec_typ'
-}.
-split.
-simpl.
-
-Ltac pmap_lookup'_simpl :=
-  repeat (
-    match goal with 
-    | H : match pmap_lookup' Empty ?p with | _Some _ => _ | _None => Empty_set end |- _ => 
-      exfalso; clear -H; rewrite pmap_lookup'_Empty in H; destruct H
-    | H : match pmap_lookup' _ ?p with | _Some _ => _ | _None => Empty_set end |- _ => 
-      destruct p; simpl in H
-    end).
-
-Definition typ'_dec {n} (a : typ' n) : forall b, {a = b} + {a <> b}.
-Proof.
-  intros.
-  destruct a as [a1 v1].
-  destruct b as [a2 v2].
-  unfold typ_map, list_to_pmap in *. simpl in *.
-  pmap_lookup'_simpl; try eq_dec_right.  
-  pose proof (base_typ_dec v1 v2).
-  destruct H; [left; subst; reflexivity|].
-  right; intros H; apply n0; inv_all; subst.
-  assert (x = eq_refl) by (apply UIP_refl); subst. reflexivity.
-  pose proof (java_typ_dec v1 v2).
-  destruct H; [left; subst; reflexivity|].
-  right; intros H; apply n0; inv_all; subst.
-  assert (x = eq_refl) by (apply UIP_refl); subst. reflexivity.
-  pose proof (list_typ_dec v1 v2).
-  destruct H; [left; subst; reflexivity|].
-  right; intros H; apply n0; inv_all; subst.
-  assert (x = eq_refl) by (apply UIP_refl); subst. reflexivity.
-  pose proof (prod_typ_dec v1 v2).
-  destruct H; [left; subst; reflexivity|].
-  right; intros H; apply n0; inv_all; subst.
-  assert (x = eq_refl) by (apply UIP_refl); subst. reflexivity.
+Global Instance RTypeOk_typ : RTypeOk. 
+apply RTypeOk_mtyp. 
 Defined.
 
-Definition typ'D {n} (t : typ' n) : type_for_arity n.
-unfold typ', typ_map, list_to_pmap in t; simpl in t.
-destruct t as [p v].
-pmap_lookup'_simpl.
-apply base_typD; assumption.
-apply java_typD; assumption.
-apply list_typD; assumption.
-apply prod_typD; assumption.
-Defined.
-
-
-Global Instance TypeView_prod_typ' : FuncView (typ' 2) (prod_typ 2) :=
-  FuncViewPMap 1 (typ_map 2) eq_refl.
+Global Instance TypeView_prod_typ' : PartialView (typ' 2) (prod_typ 2) :=
+  PartialViewPMap_Type 1 typ_map eq_refl 2.
   
-Global Instance TypeView_list_typ' : FuncView (typ' 1) (list_typ 1) :=
-  FuncViewPMap 2 (typ_map 1) eq_refl.
+Global Instance TypeView_list_typ' : PartialView (typ' 1) (list_typ 1) :=
+  PartialViewPMap_Type 2 typ_map eq_refl 1.
   
-Global Instance TypeView_base_typ' : FuncView (typ' 0) (base_typ 0) :=
-  FuncViewPMap 3 (typ_map 0) eq_refl.
+Global Instance TypeView_base_typ' : PartialView (typ' 0) (base_typ 0) :=
+  PartialViewPMap_Type 3 typ_map eq_refl 0.
   
-Global Instance TypeView_java_typ' : FuncView (typ' 0) (java_typ 0) :=
-  FuncViewPMap 4 (typ_map 0) eq_refl.
+Global Instance TypeView_java_typ' : PartialView (typ' 0) (java_typ 0) :=
+  PartialViewPMap_Type 4 typ_map eq_refl 0.
   
-Instance TypeView_prod_typ : FuncView typ (prod_typ 2 * typ * typ).
-eapply FuncView_trans. 
-apply FuncView_sym2.
-eapply (@FuncView_prod _ _ _ _ (@FuncView_prod _ _ _ _ _ FuncView_id) FuncView_id). 
+Global Instance TypeView_prod_typ : PartialView typ (prod_typ 2 * (typ * typ)).
+eapply PartialView_trans. 
+apply TypeView_sym2.
+eapply (@PartialView_prod _ _ _ _ _ PartialView_id).
 Defined.
 
-Instance TypeView_list_typ : FuncView typ (list_typ 1 * typ).
-eapply FuncView_trans. 
-apply FuncView_sym1.
-eapply (@FuncView_prod _ _ _ _ _ FuncView_id). 
+Global Instance TypeView_list_typ : PartialView typ (list_typ 1 * typ).
+eapply PartialView_trans. 
+apply TypeView_sym1.
+eapply (@PartialView_prod _ _ _ _ _ PartialView_id). 
 Defined.
 
-Instance TypeView_base_typ : FuncView typ (base_typ 0).
-eapply FuncView_trans. 
-eapply FuncView_sym0.
+Global Instance TypeView_base_typ : PartialView typ (base_typ 0).
+eapply PartialView_trans. 
+eapply TypeView_sym0.
 apply TypeView_base_typ'.
 Defined.
 
-Instance TypeView_java_typ : FuncView typ (java_typ 0).
-eapply FuncView_trans. 
-eapply FuncView_sym0.
+Global Instance TypeView_java_typ : PartialView typ (java_typ 0).
+eapply PartialView_trans. 
+eapply TypeView_sym0.
 apply TypeView_java_typ'.
+Defined.
+
+Require Import MirrorCore.Views.TypeView.
+
+Definition TypeViewOk_prod_typ
+: TypeViewOk typD (fun x => (prod_typD (n:=2) (fst x)) (typD (fst (snd x))) (typD (snd (snd x))))
+             TypeView_prod_typ.
+Proof.
+  eapply PartialView_transOk.
+  eapply TypeViewOk_sym2.
+  About PartialView_prodOk.
+  Arguments PartialView_prodOk {_ _ _ _ _ _ _ _} _ _ : clear implicits.
+  eapply PartialView_prodOk.
+  eapply PartialViewOk_TSymOneOf with (p := 1%positive) (H := TSymAll_typ_map).
+  eapply PartialViewOk_id; eapply eq_Reflexive.
+  unfold type_equiv. inversion 2.
+  etransitivity.
+  eapply H.
+  simpl in *. simpl in *. rewrite H1. rewrite H2. reflexivity.
+Defined.
+
+Definition TypeViewOk_list_typ
+: TypeViewOk typD (fun x => (list_typD (n:=1) (fst x)) (typD (snd x)))
+             TypeView_list_typ.
+Proof.
+  eapply PartialView_transOk.
+  eapply TypeViewOk_sym1.
+  About PartialView_prodOk.
+  Arguments PartialView_prodOk {_ _ _ _ _ _ _ _} _ _ : clear implicits.
+  eapply PartialView_prodOk.
+  eapply PartialViewOk_TSymOneOf with (p := 2%positive) (H := TSymAll_typ_map).
+  About PartialViewOk_id.
+  eapply PartialViewOk_id; eapply eq_Reflexive.
+  unfold type_equiv. inversion 2.
+  etransitivity.
+  eapply H.
+  simpl in *. simpl in *. rewrite H1. rewrite H2. reflexivity.
+Defined.
+
+Definition TypeViewOk_base_typ : TypeViewOk typD (@base_typD 0) TypeView_base_typ.
+eapply PartialView_transOk.
+eapply TypeViewOk_sym0.
+eapply PartialViewOk_TSymOneOf with (p := 3%positive) (H := TSymAll_typ_map).
+simpl; intros. unfold type_equiv in *.
+etransitivity; [apply H|apply H0].
+Defined.
+
+Definition TypeViewOk_java_typ : TypeViewOk typD (@java_typD 0) TypeView_java_typ.
+eapply PartialView_transOk.
+eapply TypeViewOk_sym0.
+eapply PartialViewOk_TSymOneOf with (p := 4%positive) (H := TSymAll_typ_map).
+simpl; intros. unfold type_equiv in *.
+etransitivity; [apply H|apply H0].
 Defined.
 
 Arguments tyArr {_} _ _.
@@ -179,37 +236,27 @@ Notation "'tyStringList'" := (tyList tyString).
 Notation "'tyDExprList'" := (tyList tyExpr).
 Notation "'tySubstList'" := (tyList (tyProd tyString tyExpr)).
 
-Instance TSym_typ' : TSym typ' := { 
-  symbolD := @typ'D; 
-  symbol_dec := @typ'_dec 
-}.
-
-
-(* Instantiate the RType interface *)
-Instance RType_typ : RType typ := RType_mtyp typ' _.
-Instance RTypeOk_typ : RTypeOk := @RTypeOk_mtyp typ' _.
-
 (* Build instances for describing functions and Prop *)
-Instance Typ2_tyArr : Typ2 RType_typ Fun := Typ2_Fun.
-Instance Typ2Ok_tyArr : Typ2Ok Typ2_tyArr := Typ2Ok_Fun.
+Global Instance Typ2_tyArr : Typ2 RType_typ Fun := Typ2_Fun.
+Global Instance Typ2Ok_tyArr : Typ2Ok Typ2_tyArr := Typ2Ok_Fun.
 
-Instance Typ0_tyProp : Typ0 RType_typ Prop := Typ0_sym tyProp.
-Instance Typ0Ok_tyProp : Typ0Ok Typ0_tyProp := Typ0Ok_sym tyProp.
+Global Instance Typ0_tyProp : Typ0 RType_typ Prop := Typ0_sym tyProp.
+Global Instance Typ0Ok_tyProp : Typ0Ok Typ0_tyProp := Typ0Ok_sym tyProp.
 
-Instance Typ0_tyNat : Typ0 RType_typ nat := Typ0_sym tyNat.
-Instance Typ0Ok_tyNat : Typ0Ok Typ0_tyNat := Typ0Ok_sym tyNat.
+Global Instance Typ0_tyNat : Typ0 RType_typ nat := Typ0_sym tyNat.
+Global Instance Typ0Ok_tyNat : Typ0Ok Typ0_tyNat := Typ0Ok_sym tyNat.
 
-Instance Typ0_tyString : Typ0 RType_typ string := Typ0_sym tyString.
-Instance Typ0Ok_tyString : Typ0Ok Typ0_tyString := Typ0Ok_sym tyString.
+Global Instance Typ0_tyString : Typ0 RType_typ string := Typ0_sym tyString.
+Global Instance Typ0Ok_tyString : Typ0Ok Typ0_tyString := Typ0Ok_sym tyString.
 
-Instance Typ0_tyBool : Typ0 RType_typ bool := Typ0_sym tyBool.
-Instance Typ0Ok_tyBool : Typ0Ok Typ0_tyBool := Typ0Ok_sym tyBool.
+Global Instance Typ0_tyBool : Typ0 RType_typ bool := Typ0_sym tyBool.
+Global Instance Typ0Ok_tyBool : Typ0Ok Typ0_tyBool := Typ0Ok_sym tyBool.
 
-Instance Typ1_tyList : Typ1 RType_typ plist := Typ1_sym (f_insert tList).
-Instance Typ1Ok_tyList : Typ1Ok Typ1_tyList := Typ1Ok_sym (f_insert tList).
+Global Instance Typ1_tyList : Typ1 RType_typ list := Typ1_sym (f_insert tList).
+Global Instance Typ1Ok_tyList : Typ1Ok Typ1_tyList := Typ1Ok_sym (f_insert tList).
 
-Instance Typ2_tyProd : Typ2 RType_typ prod := Typ2_sym (f_insert tProd).
-Instance Typ2Ok_tyProd : Typ2Ok Typ2_tyProd := Typ2Ok_sym (f_insert tProd).
+Global Instance Typ2_tyProd : Typ2 RType_typ prod := Typ2_sym (f_insert tProd).
+Global Instance Typ2Ok_tyProd : Typ2Ok Typ2_tyProd := Typ2Ok_sym (f_insert tProd).
 
 
 
@@ -306,21 +353,19 @@ Definition ilops : @logic_ops typ RType_typ.
                 end eq_refl
             end eq_refl
         end eq_refl).
-    + assert (f_insert p = t) by admit.  (* This is fv_ok which we do not yet have. *)
-      subst. simpl in *. apply _.
-    + assert (f_insert p = t) by admit.  (* This is fv_ok which we do not yet have. *)
-      subst. simpl in *. apply _.
-    + assert (f_insert p = t) by admit.  (* This is fv_ok which we do not yet have. *)
-      subst. simpl in *. apply _. 
-    + assert (f_insert p1 = t1) by admit.  (* This is fv_ok which we do not yet have. *)
-      assert (f_insert p2 = t2) by admit.  (* This is fv_ok which we do not yet have. *)
-      assert (f_insert p3 = t3) by admit.  (* This is fv_ok which we do not yet have. *)
-      subst; simpl in *. apply _.
-    + assert (f_insert p1 = t1) by admit.  (* This is fv_ok which we do not yet have. *)
-      assert (f_insert p2 = t2) by admit.  (* This is fv_ok which we do not yet have. *)
-      assert (f_insert p3 = t3) by admit.  (* This is fv_ok which we do not yet have. *)
-      subst; simpl in *. apply _.
-  Admitted.
+      + subst; simpl in *; forward; inversion H1; subst; inversion pf; subst.
+        pose proof (asNth_eq _ _ H0); subst; simpl; apply _.
+      + subst; simpl in *; forward. inversion H3; subst; inversion pf; subst.
+        pose proof (asNth_eq _ _ H0); subst; simpl; apply _.
+      + subst; simpl in *; forward. inversion H3; subst; inversion pf; subst.
+        pose proof (asNth_eq _ _ H0); subst; simpl; apply _.
+      + subst; simpl in *; forward. 
+        inversion pft1; inversion pft0; inversion H7; inversion pf; inversion H4; inversion H1;
+        subst; simpl in *.
+        pose proof (asNth_eq _ _ H6); pose proof (asNth_eq _ _ H0); pose proof (asNth_eq _ _ H3).
+        subst; simpl. apply _.
+      + subst; simpl in *; forward. 
+Defined.
 
   Definition bilops : @bilogic_ops _ RType_typ.
   refine (
@@ -373,13 +418,10 @@ Definition ilops : @logic_ops typ RType_typ.
             | _ => fun _ => pNone
             end eq_refl 
         end eq_refl).
-  + assert (f_insert p = t) by admit.  (* This is fv_ok which we do not yet have. *)
-    subst. simpl in *. apply _.
-  + assert (f_insert p1 = t1) by admit.  (* This is fv_ok which we do not yet have. *)
-    assert (f_insert p2 = t2) by admit.  (* This is fv_ok which we do not yet have. *)
-    assert (f_insert p3 = t3) by admit.  (* This is fv_ok which we do not yet have. *)
-    subst; simpl in *. apply _.
-  Admitted.
+  + subst; simpl in *; forward; inversion H1; inversion pf; subst.
+    pose proof (asNth_eq _ _ H0); subst; simpl; apply _.
+  + subst; simpl in *; forward; inversion H1; inversion pf; subst.
+Defined.
 
 (*
 Definition eops : @embed_ops _ RType_typ :=
