Java/src/Java/Language/Program.v
@@ -4,6 +4,293 @@ Require Import Lang Util.
 Require Import ExtLib.Core.RelDec.
 Require Import ExtLib.Tactics.Consider.
 
+Require Import ExtLib.Data.Pair.
+Require Import ExtLib.Data.List.
+
+Set Implicit Arguments.
+Unset Strict Implicit.
+
+Section RelDecNoDup.
+  Require Import Coq.Bool.Bool.
+  
+  Context {A : Type} {RelDec_A : RelDec (@eq A)} 
+	  {RelDec_Correct_A : RelDec_Correct RelDec_A}.
+  
+  Fixpoint inb (x : A) (lst : list A) := 
+    match lst with
+    | nil => false
+    | l::ls => if x ?[ eq ] l then true else inb x ls
+    end.
+	  
+  Lemma inb_sound (x : A) (lst : list A) (H : inb x lst = true) : In x lst.
+  Proof.
+    induction lst; simpl in *; try congruence.
+    consider (x ?[ eq ] a); intros; subst.
+    + left; reflexivity.
+    + right; apply IHlst; assumption.
+  Qed.
+  
+  Lemma inb_complete (x : A) (lst : list A) (H : In x lst) : inb x lst = true.
+  Proof.
+    induction lst; simpl in *; try intuition congruence.
+    consider (x ?[ eq ] a); intros; destruct H as [H | H]; try congruence.
+    apply IHlst; assumption.
+  Qed.
+  
+  Fixpoint nodup (lst : list A) : bool :=
+    match lst with
+    | nil => true
+    | l :: ls => (negb (inb l ls) && nodup ls)%bool
+    end.
+  
+  Lemma nodup_sound (lst : list A) (H : nodup lst = true) : NoDup lst.
+  Proof.
+    induction lst.
+    + constructor.
+    + simpl in *. rewrite andb_true_iff in H; destruct H as [H1 H2].
+      rewrite negb_true_iff in H1. constructor.
+      * intro H. apply inb_complete in H. intuition congruence.
+      * apply IHlst; assumption.
+  Qed.
+	  	
+  Lemma nodup_complete (lst : list A) (H : NoDup lst) : nodup lst = true.
+  Proof.
+    induction lst.
+    + constructor.
+    + simpl in *. rewrite andb_true_iff. inversion H; subst; split; clear H.
+      * apply eq_true_not_negb. intros H; apply H2. apply inb_sound; assumption.
+      * apply IHlst; assumption.
+  Qed.
+  
+End RelDecNoDup.
+
+Record Method := {
+  m_params: list var;
+  m_body: cmd;
+  m_ret: dexpr
+}.
+
+Instance RelDec_Method : RelDec (@eq Method) := {
+	rel_dec m1 m2 := (m_params m1 ?[ eq ] m_params m2 &&
+					  m_body m1 ?[ eq ] m_body m2 &&
+					  m_ret m1 ?[ eq ] m_ret m2)%bool
+}.
+
+Instance RelDec_Correct_Method : RelDec_Correct RelDec_Method.
+Proof.
+	split; intros; destruct x, y; simpl.
+	consider (m_params0 ?[ eq ] m_params1);
+	consider (m_body0 ?[ eq ] m_body1);
+	consider (m_ret0 ?[ eq ] m_ret1); simpl; intuition congruence.
+Qed.
+
+Record Class := {
+  c_fields  : list field;
+  c_methods : list (string * Method)
+}.
+
+Instance RelDec_Class : RelDec (@eq Class) := {
+	rel_dec c1 c2 := (c_fields c1 ?[ eq ] c_fields c2 &&
+					  c_methods c1 ?[ eq ] c_methods c2)%bool
+}.
+
+Instance RelDec_Correct_Class : RelDec_Correct RelDec_Class.
+Proof.
+	split; intros; destruct x, y; simpl.
+	consider (c_fields0 ?[ eq ] c_fields1);
+	consider (c_methods0 ?[ eq ] c_methods1); intros;
+		 simpl; try intuition congruence.
+Qed.
+
+Record Program := {
+  p_classes: list (string * Class)
+}.
+
+Instance RelDec_Program : RelDec (@eq Program) := {
+  rel_dec p1 p2 := (p_classes p1) ?[ eq ] (p_classes p2)
+}.
+
+Instance RelDec_Correct_Program : RelDec_Correct RelDec_Program.
+Proof.
+	split; intros; destruct x, y; simpl.
+	consider (p_classes0 ?[ eq ] p_classes1); intuition congruence.
+Qed.
+
+Definition valid_method (M : Method) := nodup (m_params M).
+
+Definition valid_class (C : Class) : bool :=
+	let (names, methods) := split (c_methods C) in
+	nodup (c_fields C) && nodup names &&
+	  forallb (fun M => valid_method M) methods.
+
+Definition valid_program (P : Program) : bool :=
+	let (names, classes) := split (p_classes P) in
+	    nodup names &&
+		forallb valid_class classes.
+
+Fixpoint class_lookup_aux C (lst : list (string * Class)) :=
+	match lst with
+		| nil => None
+		| (c, Crec)::ls => if C ?[ eq ] c then Some Crec else class_lookup_aux C ls
+	end.
+
+Definition class_lookup C P := class_lookup_aux C (p_classes P).
+
+Lemma split_Prop {A B C : Type} (lst : list (A * B)) (P : list A -> list B -> C) : 
+	(let (a, b) := split lst in P a b) =
+	P (fst (split lst)) (snd (split lst)).
+Proof.
+  generalize dependent C.
+  induction lst; try reflexivity; intros; destruct a; simpl.
+  replace (let (g, d) := split lst in (a :: g, b :: d)) with
+  		  (a :: fst (split lst), b :: snd (split lst)) by (symmetry; apply IHlst).
+  reflexivity.
+Qed.
+
+Section Pwf.
+
+  Variable Prog: Program.
+  Variable (Valid : valid_program Prog = true).
+
+  Definition field_lookup (C:class) (fields: list field) :=
+  	exists Crec, In (C, Crec) (p_classes Prog) /\
+  		fields = c_fields Crec.
+
+  Lemma field_lookup_function C f f' 
+  	(H1 : field_lookup C f) (H2 : field_lookup C f') : f = f'. 
+  Proof.
+    unfold field_lookup in *.
+    destruct H1 as [m [H11 H12]]; destruct H2 as [n [H21 H22]].
+    unfold valid_program in Valid. simpl in *.
+    assert (m = n); [|subst; reflexivity].
+    rewrite split_Prop, andb_true_iff in Valid.
+    destruct Valid; clear Valid.
+    induction (p_classes Prog); simpl in *; try intuition congruence.
+    destruct a; simpl in *.
+    rewrite split_Prop in H, H0; simpl in *; rewrite andb_true_iff in H, H0.
+    destruct H, H0.
+    rewrite negb_true_iff in H.
+    destruct H11, H21.
+    + inversion H3; inversion H4; subst; apply H9.
+    + inversion H3; subst; clear IHl.
+      assert (~inb C (fst (split l)) = true) by (unfold class; intuition congruence).
+	  contradiction H5; clear H H5.
+	  apply inb_complete.
+	  apply in_split_l in H4. apply H4.
+	+ inversion H4; subst; clear IHl.
+      assert (~inb C (fst (split l)) = true) by (unfold class; intuition congruence).
+	  contradiction H5; clear H H5.
+	  apply inb_complete.
+	  apply in_split_l in H3. apply H3.
+    + apply IHl; try assumption.
+  Qed.
+
+  Definition method_lookup (C:class) m mrec :=
+    exists Crec, In (C, Crec) (p_classes Prog) /\
+      In (m, mrec) (c_methods Crec).
+
+  Lemma method_lookup_function : forall C m mr0 mr1
+    (HML0 : method_lookup C m mr0)
+    (HML1 : method_lookup C m mr1),
+    mr0 = mr1.
+  Proof.
+    unfold Pwf.method_lookup; intros; destruct HML0 as [C0 [HC0 HM0]];
+      destruct HML1 as [C1 [HC1 HM1]].
+   unfold valid_program in Valid. simpl in *.
+    rewrite split_Prop, andb_true_iff in Valid.
+    destruct Valid; clear Valid.
+    induction (p_classes Prog); simpl in *; try intuition congruence.
+    destruct a; simpl in *.
+    rewrite split_Prop in H, H0; simpl in *; rewrite andb_true_iff in H, H0.
+    destruct H, H0.
+    rewrite negb_true_iff in H.
+    destruct HC0, HC1.
+    + clear IHl; inversion H3; inversion H4. repeat subst; clear H H1 H2 H3 H4 H8.
+	  unfold valid_class in H0. rewrite split_Prop in H0; repeat rewrite andb_true_iff in H0.
+	  destruct H0 as [[_ H] _].
+	  induction (c_methods C1); simpl in *; try intuition congruence.
+	  destruct a; rewrite split_Prop in H; simpl in H.
+	  rewrite andb_true_iff in H; destruct H as [H1 H2].
+	  rewrite negb_true_iff in H1.
+	  destruct HM1, HM0.
+	  * inversion H; inversion H0; repeat subst; reflexivity.
+	  * inversion H; subst; clear IHl0.
+        assert (~inb m (fst (split l0)) = true) by intuition congruence.
+        contradiction H3. apply inb_complete.
+        apply in_split_l in H0; apply H0.
+	  * inversion H0; subst; clear IHl0.
+        assert (~inb m (fst (split l0)) = true) by intuition congruence.
+        contradiction H3. apply inb_complete.
+        apply in_split_l in H; apply H.
+	  * apply IHl0; assumption.
+    + inversion H3; subst; clear IHl.
+      assert (~inb C (fst (split l)) = true) by (unfold class; intuition congruence).
+	  contradiction H5; clear H H5.
+	  apply inb_complete.
+	  apply in_split_l in H4. apply H4.
+	+ inversion H4; subst; clear IHl.
+      assert (~inb C (fst (split l)) = true) by (unfold class; intuition congruence).
+	  contradiction H5; clear H H5.
+	  apply inb_complete.
+	  apply in_split_l in H3. apply H3.
+    + apply IHl; try assumption.
+  Qed.
+
+  Lemma method_lookup_nodup C m mr (H : method_lookup C m mr) : NoDup (m_params mr).
+  Proof.
+    unfold method_lookup in H.
+    destruct H as [Crec [H1 H2]].
+    unfold valid_program in Valid.
+    rewrite split_Prop, andb_true_iff in Valid.
+    destruct Valid as [H3 H4]; clear Valid.
+	induction (p_classes Prog); simpl in *; try intuition congruence.
+	destruct a; rewrite split_Prop in H3; simpl in *.
+	rewrite andb_true_iff in H3; destruct H3 as [H3 H5].
+	rewrite negb_true_iff in H3.
+	rewrite split_Prop in H4; simpl in *.
+	rewrite andb_true_iff in H4; destruct H4 as [H4 H6].
+	unfold valid_class in H4. rewrite split_Prop in H4; repeat rewrite andb_true_iff in H4.
+	destruct H4 as [[H4 _] H7].
+	destruct H1 as [H1 | H1]; [
+		inversion H1; repeat subst; clear H1 IHl|
+		apply IHl; assumption
+	].
+	clear H3 H4 H5 H6 l C Prog.
+	induction (c_methods Crec); simpl in *; try intuition congruence.
+	destruct a; simpl in *; rewrite split_Prop in H7; simpl in *.
+	rewrite andb_true_iff in H7; destruct H7 as [H1 H3].
+	destruct H2 as [H2 | H2]; [|apply IHl; assumption].
+	inversion H2; subst; clear H2 H3 IHl.
+	unfold valid_method in H1. apply nodup_sound; assumption.
+Qed.
+
+End Pwf.
+
+Definition Prog_compat (P Q : Program) :=
+  forall C, ~ (In C (p_classes P) /\ In C (p_classes Q)).
+
+Definition Prog_sub (P Q : Program) :=
+  forall C crec, In (C, crec) (p_classes P) ->
+    exists crec', In (C, crec') (p_classes Q) /\
+      c_fields crec = c_fields crec' /\
+      c_methods crec = c_methods crec'.
+
+Instance Prog_sub_preo : PreOrder Prog_sub.
+Proof.
+  split.
+  + intros P x C HF; exists C; repeat split; trivial.
+  + intros P Q R HPQ HQR x C HF.
+  destruct (HPQ _ _ HF) as [D [HLu [HFs HMs]]].
+  destruct (HQR _ _ HLu) as [E [HLuR [HFs' HMs']]].
+  exists E; split; [assumption | split; etransitivity; eassumption].
+Qed.
+(*
+Require Import List Coq.Strings.String RelationClasses Morphisms Setoid.
+Require Import Lang Util.
+
+Require Import ExtLib.Core.RelDec.
+Require Import ExtLib.Tactics.Consider.
+
 Require Import ExtLib.Data.PPair.
 Require Import ExtLib.Data.PList.
 Require Import ExtLib.Data.String.
@@ -253,3 +540,4 @@ Proof.
   destruct (HQR _ _ HLu) as [E [HLuR [HFs' HMs']]].
   exists E; split; [assumption | split; etransitivity; eassumption].
 Qed.
+*)
